---
{"dg-publish":true,"permalink":"/Advanced Math 高等数学/6_多元函数/例题：求极限/","tags":["微积分","例题"]}
---

#### 换元为一元极限

> [!Question] 问题
> $$
> \lim_{ (x,y) \to (0,0)}  \frac{24\cos \sqrt{ x^{2} + y^{2} } - 24  + 12(x^{2} + y ^{2})}{(\tan \sqrt{ x^{2} + y^{2} })^{4}}
> $$

令$r = \sqrt{ x^{2} + y^{2} }$
则
$$
\begin{align}
 & \lim_{ r \to 0 } \frac{24\cos r - 24 + 12r^{2}}{(\tan r)^{4}} \\
\end{align}
$$
做等价无穷小代换
$$
\begin{align}
 & \lim_{ r \to 0 } \frac{24\cos r - 24 + 12r^{2}}{r^{4}}  \\
\text{洛} & =  \lim_{ r \to 0 } \frac{ -24\sin r  + 24r}{4r^{3}} \\
& =  \lim_{ r \to 0 } \frac{ -6\sin r  + 6r}{r^{3}} \\
\text{洛}& =  \lim_{ r \to 0 } \frac{ -6\cos r  + 6}{3r^{2}} \\
\text{洛}& =  \lim_{ r \to 0 } \frac{ -2\cos r  + 2}{r^{2}} \\
\text{洛}& =  \lim_{ r \to 0 } \frac{ 2\sin r }{2r} \\
 & = 1
\end{align}
$$

#### 综合

> [!Question] 问题
> $$
> \lim_{ (x,y) \to (0,0)}  xy\ln(x^{2} + y^{2})
> $$


先对$xy$做放缩
$$
|xy| \leq \frac{1}{2}(x^{2} + y^{2})
$$
那么
$$
0 \leq |xy\ln (x^{2} + y^{2})| \leq \frac{1}{2}(x^{2} + y^{2})|\ln(x^{2} + y^{2})|
$$
可以看到有函数只剩下$x^{2} + y^{2}$，做换元
$$
\begin{align}
t = x^{2} + y^{2} , (x,y) \to (0,0) , t \to 0 \\
\frac{1}{2}(x^{2} + y^{2})|\ln(x^{2} + y^{2})| = \frac{1}{2}|t \ln t|
\end{align}

$$


因此变为求
$$
\begin{align}
\lim_{ t \to 0 } t\ln t  & = \lim_{ t \to 0 } \frac{\ln t}{\frac{1}{t}} \\
\text{洛}  & = \lim_{ t \to 0 } \frac{\frac{1}{t}}{-\frac{1}{t^{2}}} \\
 & = \lim_{ t \to 0 }- t \\
 & = 0
\end{align}
$$
由夹逼准则，
$$
\lim_{ (x,y) \to (0,0)}  xy\ln(x^{2} + y^{2}) = 0
$$

> [!Question] 问题
> 证明极限不存在
> $$
> \lim_{ (x,y) \to (0,0)}   \left( \frac{xy}{e^{x} - 1} + \sin y  \right)\sin \frac{1}{x^{2} + y^{2}}
> $$

$$
 0<|\left( \frac{xy}{e^{x} - 1} + \sin y  \right)\sin \frac{1}{x^{2} + y^{2}}| \leq | \frac{xy}{e^{x} - 1} + \sin y |
$$
而
$$
\begin{align}
 & \lim_{ (x,y) \to (0,0) } \frac{xy}{e^{x } - 1}  \\
 & = \lim_{ (x,y) \to (0,0) } \frac{xy}{x} \left( \frac{x}{e^{x } - 1} \right)  \\
 & = \lim_{ y \to 0 } y \lim_{ x \to 0 } \frac{x}{e^{x}-1}  \\
 & =\lim_{ y \to 0 } y \lim_{ x \to 0 } \frac{1}{e^{x}}  \\
 & =\lim_{ y \to 0 } y  \\
 & =0
\end{align}
$$
且
$$
\lim_{ y \to 0 } \sin y = 0
$$
则由于夹逼准则
$$
\lim_{ (x,y) \to (0,0)}   \left( \frac{xy}{e^{x} - 1} + \sin y  \right)\sin \frac{1}{x^{2} + y^{2}} = 0
$$
