---
{"dg-publish":true,"permalink":"/Advanced Math 高等数学/9_微分方程/例题/例题：二阶常系数线性微分方程/","tags":["高数","微积分","例题"]}
---


## 齐次线性微分方程

> [!Question] 例题
> 求通解$y^{\prime\prime}-2y^{\prime} - 3y =0$

特征方程为
$$
\begin{align}
r^{2} -2 r -3 =0
(r-3)(r+1) = 0 \\
r_{1} = 3 , r_{2} = -1
\end{align}
$$
则通解为$y = C_{1}e^{ 3x} + C_{2}e^{-x}$

求特解
$$
\begin{cases}
y^{\prime\prime}+2y^{\prime} + y =0 \\
y|_{x=0} = 4, y^{\prime}|_{x=0} = -2 
\end{cases}
$$
特征方程：
$$
\begin{align}
r^{2} + 2r + 1 = 0 \\
(r+1)^{2} = 0 \\
r_{1} = r_{2} = -1
\end{align}
$$
则通解为
$$
y = (C_{1} + C_{2}x)e^{-x}
$$

当$x = 0,y=4$
$$
C_{1} = 4
$$
当$x=0 , y^{\prime} =-2$
$$
\begin{align}
y^{\prime} &  = C_{2}e^{-x} - (C_{1} + C_{2}x) e^{-x} \\
-2 & =C_{2}-C_{1}\\
C_{2}  & = 2
\end{align}
$$
特解为
$$
y^{*} = (4 + 2x)e^{-x}
$$

> [!Question] 例题
> 求通解$y^{\prime\prime} -2y^{\prime} + 5 = 0$
> 

$$
\begin{align}
r^{\prime\prime} -2r^{\prime} + 5 = 0 \\
(r-1)^{2} + 4 = 0 \\
(r-1) = \pm2 i \\
r_{1} =1+ 2i , r_{2} = 1- 2i \\
\alpha = 1 , \beta =2
\end{align}
$$
则
$$
\begin{align}
y &  = e^{\alpha x}(c_{1}\cos \beta x + C_{2} \sin \beta x) \\
 & = e^{x}(C_{1} \cos 2x + C_{2} \sin 2x)
\end{align}
$$

## 非齐次线性微分方程

#### 待定系数法

求$y^{\prime\prime}-2y^{\prime} - 3y = 3x + 1$的通解

**找齐次通解**

特征方程：
$$
\begin{align}
r^{2}-2r - 3 = 0 \\
(r-3)(r+1) = 0 \\
r_{1} = 3, r_{2} = -1
\end{align}
$$
则齐次线性微分方程$y^{\prime\prime}-2y^{\prime} - 3y =0$的通解为$C_{1}e^{2x}+C_{2}e^{-x}$

**非齐次特解**
$y^{\prime\prime}-2y^{\prime} - 3y = e^{\lambda x}P_{m}(x)$
由$3x + 1$推出$\lambda=0,m=1$
由于$\lambda \ne r_{1} ,\lambda\ne r_{2}$，$\lambda$与$0$个$r$相等$\to k= 0$

设特解$y^{*} = e^{\lambda x}(ax +b)x^{k}$
则
$y^{*} = ax + b$
将上式代入微分方程
得
$$
\begin{align}
-2a -3(ax + b) = 3x + 1 \\
-3ax -2a - 3b = 3x +1
\end{align}
$$
得$a = -1,b = \frac{1}{3}$

因此$y^{*} = -x + \frac{1}{3}$

通解为$y = C_{1}e^{2x}+C_{2}e^{-x} -x + \frac{1}{3}$

> [!Question] 例题
> 求通解$y^{\prime\prime}-5y^{\prime}  + 6y = xe^{2x}$

**找齐次通解**
$$
\begin{align}
r^{2} -5r + 6 = 0 \\
(r-3)(r-2) = 0 \\
r_{1} = 3 , r_{2} = 2
\end{align}
$$
则齐次线性微分方程$解$$y^{\prime\prime}-5y^{\prime}  + 6y=0$的通解为$C_{1}e^{3x} + C_{2}e^{2x}$

**非齐次特解**
$y^{\prime\prime}-5y^{\prime}  + 6y= e^{\lambda x}P_{m}(x)$
得
$$
\begin{cases}
\lambda = 2 \\
m = 1
\end{cases}
$$
且$\lambda\ne r_{1} ,\lambda = r_{2}$，$\lambda$有$1$个$r$相等，$k =1$
特解为
$$
\begin{align}
y^{*} &  = e^{\lambda x}(ax +b)x^{1} \\
 & =e^{2x}(ax^{2} + bx)
\end{align}
$$
将$y^{*}$代入微分方程
已知
$$
\begin{cases}
y^{*\prime} =2e^{2x}(ax^{2} + bx) + e^{2x}(2ax + b) = (2ax^{2} + 2(a+b)x + b)e^{2x}\\
(y^{*})^{\prime\prime}=2e^{2x}(2ax^{2} + 2(a+b)x + b) + e^{2x}(4ax + 2(a+b)) =(4ax^{2} +(8a + 4b)x + 2a + 4b)e^{2x}\\
\end{cases}
$$

$$
\begin{align}
y^{\prime\prime}-5y^{\prime}  + 6y = xe^{2x} \\
(4ax^{2} +(8a + 4b)x + 2a + 4b)e^{2x} -5(2ax^{2} + 2(a+b)x + b)e^{2x} +6e^{2x}(ax^{2} + bx) =xe^{x} \\
-2ax + 2a - b = x \\
\end{align}
$$
得
$$
\begin{cases}
a = -\frac{1}{2} \\
b = -1
\end{cases}
$$
则$y^{*} = e^{2x}\left( -\frac{1}{2}x^{2} -x \right)$

通解为$C_{1}e^{3x} + C_{2}e^{2x} +\left( -\frac{1}{2}x^{2} -x \right)e^{2x}$

求通解$y^{\prime\prime}-2y^{\prime} + y = (3x + 2)e^{x}$

$$
\begin{align}
r^{2} - 2r + 1 = 0 \\
(r-1)^{2} = 0 \\
r_{1} = r_{2} = 1
\end{align}
$$

非齐通解为$(C_{1} + C_{2}x)e^{x}$

非齐次特解
由$y^{\prime\prime}-2y^{\prime} + y = (3x + 2)e^{x}$可知
$$
\begin{cases}
\lambda = 1 \\
m = 1
\end{cases}
$$
由于$\lambda = r_{1} = r_{2}$，$k=2$
$$
y^{*} =e^{\lambda x}(ax + b)x^{k} = e^{x}(ax + b)x^{2} = e^{x}(ax^{3} + bx^{2})
$$
则将
$$
\begin{cases}
y^{\prime}  & = e^{x}(ax^{3} + bx^{2}) + e^{x}(3ax^{2} + 2bx)  = (ax^{3} + (3a + b)x^{2} + 2bx)e^{x}\\
y^{\prime\prime}  & = (ax^{3} + (3a + b)x^{2} + 2bx)e^{x} + (3ax^{2} + 2(3a + b)x + 2b)e^{x} \\
 & =(ax^{3} +(6a + b)x^{2} + (6a + 4b)x + 2b)
\end{cases}
$$
代入微分方程
则
$$
\begin{align}
y^{\prime\prime}-2y^{\prime} + y = (3x + 2)e^{x} \\
6ax+ 2b=(3x + 2)
\end{align}
$$
则
$$
\begin{cases}
a =\frac{1}{2} \\
b = 1
\end{cases}
$$
则$y^{*} =e^{x}\left( \frac{1}{2}x^{3} + x^{2} \right)$

则通解为$y =(C_{1} + C_{2}x)e^{x} +\left( \frac{1}{2}x^{3} + x^{2} \right)e^{x}$

> [!Question] 
> 
> $y^{\prime\prime}+y = x\cos 2x$求通解
> 

**齐次通解**
$$
\begin{align}
r^{2} + 1 = 0 \\ 
r_{1} = i , r_{2}  = -i
\end{align}
$$
得$\alpha = 0 ,\beta = 1$
齐次通解为$C_{1}\cos x + C_{2}\sin x$

$y^{\prime\prime} + y = e^{\lambda x}[P_{L}(x)\cos \omega x + Q_{n}(x)\sin \omega x]$
则
$$
\begin{cases}
\lambda = 0 \\
\omega = 2 \\
L =1\\
n = 0
\end{cases}
$$
$m = max(L,n) =1$
$\lambda + \omega i =0 + 2i \ne r_{1} \ne r_{2}$
则$k = 0$

设
$$
\begin{align}
y^{*} &  = x^{k}e^{\lambda x}[R_{m_{1}}(x)\cos \omega x + R_{m_{2}}(x)\sin \omega x ] \\
 & = (ax + b)\cos 2x + (cx + d)\sin 2x
\end{align}
$$
#### 常数变易法

$$
y^{\prime\prime}-2y^{\prime} + y = \frac{e^{x}}{x}  
$$
通解
$$
\begin{align}
\lambda^{2} -2\lambda + 1 = 0
 \\
(\lambda -1)^{2} = 0 \\
\lambda_{1} = \lambda_{2} = 1
\end{align}
$$

通解为$(C_{1} + C_{2}x)e^{x}$

假设$y = C_{1}(x)e^{x} + C_{2}(x)xe^{x}$是非齐次的解

由常数变易法
$$
\begin{cases}
C_{1}^{\prime}(x)\phi_{1}(x) + C_{2}^{\prime} (x)\phi_{2}(x) = 0 \\
C_{1}^{\prime}(x)\phi_{1}^{\prime}(x)  + C_{2}^{\prime}(x)\phi_{2}^{\prime}(x) = f(x)   \\
 \\
C_{1}^{\prime}(x)e^{x} + C_{2}^{\prime} (x)xe^{x} = 0 \\
C_{1}^{\prime}(x)e^{x} + C_{2}^{\prime}(x)(1+x)e^{x} = \frac{e^{x}}{x}  
\end{cases}
$$
得
$$
\begin{cases}
C_{2}^{\prime}(x) = \frac{1}{x} \\
C_{1}^{\prime}(x) = -1 \\
 \\
C_{1}(x) = -x + C_{1} \\
C_{2}(x) =\ln x + C_{2}  
\end{cases}
$$


