---
{"dg-publish":true,"permalink":"/Advanced Math 高等数学/9_微分方程/例题/例题：齐次微分方程/","tags":["高数","微积分","例题"]}
---


> [!Question] 例题
> 求通解
> $$
> y^{2} + x^{2} \frac{dy}{dx} = xy \frac{dy}{dx}
> $$



$$
\begin{align}
y^{2} =(xy -x^{2}) \frac{dy}{dx} \\
\frac{dy}{dx} = \frac{y^{2}}{xy -x^{2}} \\
\frac{dy}{dx} = \frac{\left( \frac{y}{x} \right)^{2}}{\frac{y}{x} - 1}
\end{align}
$$

令$\frac{y}{x} = \mu$
$$
\begin{align}
\mu + x\frac{d\mu}{dx}= \frac{\mu^{2}}{\mu - 1} \\
 x\frac{d\mu}{dx} = \frac{\mu^{2}}{\mu - 1} - \frac{\mu^{2} - \mu}{\mu - 1} \\
\frac{\mu - 1}{\mu} d\mu = \frac{1}{x}dx \\
\mu - \ln \mu = \ln x + C \\
\mu = \ln Cx\mu \\
\frac{y}{x} = ln Cx\left( \frac{y}{x} \right) \\
\frac{y}{x} = \ln Cy \\
Cy = e^{y/x}
\end{align}
$$


> [!Question] 例题
> 求
> $$
> \frac{dy}{dx} = \frac{y}{x} - \frac{1}{2}\left( \frac{y}{x} \right)^{3}
> $$
> 在$y(1) = 1$的特解


$$
\begin{align}
\mu + x\frac{d\mu}{dx} = \mu - \frac{1}{2} \mu^{3}   \\
-\frac{2}{\mu^{3}}d\mu = \frac{1}{x}dx \\
\frac{1}{\mu^{2}} = \ln x  + C\\
\frac{x^{2}}{y^{2}} = \ln x + C \\
\end{align}
$$
令$x=1,y=1$
$$
C = 1
$$
则
$$
\begin{align}
\frac{x^{2}}{y^{2}} = \ln x + 1 \\
\end{align}
$$

求解微分方程$\left( 1 + e^{\frac{x}{y}} \right)dx + e^{\frac{x}{y}}\left( 1 - \frac{x}{y} \right)dy = 0$
令$u = \frac{x}{y}, \frac{dx}{dy} =u +y \frac{du}{dy}$

$$
\begin{align}
\left( 1 + e^{\frac{x}{y}} \right)dx = e^{\frac{x}{y}}\left( \frac{x}{y} - 1 \right)dy \\
\frac{dx}{dy }\left( 1 + e^{\frac{x}{y}} \right) = e^{\frac{x}{y}}\left( \frac{x}{y} - 1 \right) \\
\left( u + y \frac{du}{dy} \right)(1 + e^{u})= e^{u}(u -1) \\
y \frac{du}{dy} & =\frac{e^{u}(u-1)}{1 + e^{ u }} - u \\
 & = \frac{-e^{u}-u}{1 + e^{ u }} \\
- \frac{1 + e^{u}}{u + e^{u}} du & = \frac{1}{y}dy \\
\ln(u + e^{ u }) & =- \ln |y| + C \\
y(u + e^{ u }) & = C  \\
x + ye^{  \frac{x}{y} }  & = C
\end{align}
$$
### 换元法

> [!Question] 例题
> $y^{3}dx + 2(x^{2} - xy^{2})dy = 0$，求通解


> [!NOTE] 思路
> 使用换元，将上述方程转化为齐次方程组

令$x = \mu^{2},dx= 2\mu d\mu$

$$
\begin{align}
2\mu y^{3} d\mu  & = 2(\mu^{2}y^{2} - \mu^{4})dy \\
\frac{dy}{d\mu} &  =\frac{\mu y^{3}}{(\mu^{2}y^{2} - \mu^{4})} \\
 & = \frac{\frac{y^{3}}{\mu^{3}}}{\frac{y^{2}}{\mu^{2}} - 1} \\
\end{align}
$$
令$t = \frac{y}{\mu}$
$$
\begin{align}
t + \frac{\mu dt}{d\mu} = \frac{t^{3}}{t^{2} - 1} \\
\frac{\mu dt}{d\mu}= \frac{t^{3} - t^{3}  + t^{2}}{t^{2} - 1} \\
\left(t - \frac{1}{t} \right)dt = \frac{1}{\mu}d\mu \\
\frac{t^{2}}{2} - \ln t = \ln \mu  + C\\
\frac{1}{2}\frac{y^{2}}{\mu^{2}} - \ln y + \ln \mu= \ln \mu + C \\
\frac{1}{2}\frac{y^{2}}{\mu^{2}} - \ln y = C \\
\frac{y^{2}}{2x}-\ln y = C \\
e^{C}y =e^{y^{2}/2x}
\end{align}
$$

令$\frac{1}{e^{C}} = c_{1}$
$$
y = c_{1}e^{y^{2}/2x}
$$

#### $f(ax + by + c)$

求解常微分方程$y^{\prime} =(8x + 2y + 1)^{2}$

令$z = 8x + 2y  +1$
$$
\begin{align}
\frac{dz}{dx} = 8  + 2 \frac{dy}{dx} =8 + 2z^{2} \\
\frac{dz}{dx} & =8 + 2z^{2} \\
\frac{1}{8 + 2z^{2}}dz  & = dx \\
\frac{1}{8} \arctan \frac{z}{2}  & = x + C\\
\frac{1}{8} \arctan \left( 4x + y + \frac{1}{2} \right) & = x + C
\end{align}
$$

#### $f\left( \frac{a_{1}x + b_{1}y + c_{1}}{a_{2}x + b_{2}y + c_{2}} \right)$

##### 系数线性相关：

求解微分方程$y^{\prime} =\frac{x + 2y + 1}{2x  + 4y -1}$

令$z = x + 2y$
$$
\begin{align}
\frac{dz}{dx} = 1 + 2 \frac{dy}{dx} =1 + \frac{2( z + 1)}{2 z- 1} \\
\frac{dz}{dx} & =  \frac{4z + 1}{2z - 1} \\
\frac{2z - 1}{4z + 1} dz  & = dx \left( \text{when } z\ne -\frac{1}{4}  \right)\\
\left( 1 - \frac{3}{4z + 1} \right)  & = 2dx \\
z - \frac{3}{4}\ln |4z + 1| & = 2x + C \\
x+ 2y - \frac{3}{4}\ln |4x + 8y + 1|  & =2x + C \\
e^{8y-4x}(4x + 8y + 1)^{3}  & = C
\end{align}
$$
判断$z = -\frac{1}{4}$是否存在特解
当$z = -\frac{1}{4}$
$$
4x + 8y + 1 = 0
$$

##### 系数线性无关：

求解微分方程$y^{\prime} = 2\left( \frac{y + 2}{x + y - 1} \right)^{2}$

解方程
$$
\begin{cases}
y + 2 = 0 \\
x  + y - 1 = 0
\end{cases}
$$
得$y=-2,x=3$
则令$u=x-3,v=y +  2$
则$\frac{dy}{dx}=\frac{dv}{du}$
$$
\begin{align}
\frac{dv}{du}  & = 2\left( \frac{v}{u + v} \right)^{2} \\
\end{align}
$$
令$t = \frac{v}{u}$
$\frac{dv}{du} = t + u \frac{dt}{du}$
$$
\begin{align}
t + u \frac{dt}{du}  & = 2\left( \frac{t}{1 + t} \right)^{2} \\
u \frac{dt}{du} & = \frac{2t^{2} - t^{3} - 2t^{2} - t }{t^{2}  +2t + 1}\\
\frac{(t + 1)^{2}}{t(t^{2} + 1)} &  = -\frac{1}{u}du\\
\int \frac{t^{2} + 1}{t(t^{2} + 1)} + \frac{2t}{t(t^{2} + 1)} dt & =-\int \frac{1}{u}du \\
\ln |t|  +2 \arctan t & =- \ln |u| +c \\
ute^{2 \arctan t} & = C \\
ve^{2\arctan \frac{v}{u}}  & = C \\
(y + 2) \exp\left( 2 \arctan\left( \frac{y + 2}{x - 3} \right) \right) & = C
\end{align}
$$


