---
{"dg-publish":true,"permalink":"/Advanced Math 高等数学/9_微分方程/例题/例题：一阶线性微分方程/","tags":["高数","微积分","例题"]}
---


#### 常数变易法

> [!Question] 例题
> 求通解
> $$
> \frac{dy}{dx} - \frac{2y}{x+1} = (x+1)^{5/2}
> $$

有
$$
\begin{align}
P = -\frac{2}{x + 1} \\
Q(x) = (x + 1)^{\frac{5}{2}}
\end{align}
$$

1. 求齐次线性方程通解
$$
\begin{align}
\frac{dy}{dx} = \frac{2y}{x + 1} \\
\frac{1}{y}  dy= \frac{2}{x + 1}dx \\
\ln y = 2\ln(x+ 1) + \ln C \\
y = C(x + 1)^{2}
\end{align}
$$

2. 常数变易法求特解

令$y^{*} = \mu(x)(x+1)^{2}$
$$
\begin{align}
\frac{dy^{*}}{dx} = \mu^{\prime}(x)(x+1)^{2} + 2\mu(x)(x+1) \\
-\frac{2y^{*}}{x + 1} = -\frac{2\mu(x)(x + 1)^{2}}{x + 1} \\
-\frac{2y^{*}}{x + 1} = -2\mu(x)(x+1)
\end{align}
$$
两式相加得
$$
\begin{align}
\frac{dy^{*}}{dx} -\frac{2y^{*}}{x + 1} =  \mu^{\prime}(x)(x+1)^{2} \\
(x + 1)^{5/2}  & = \mu^{\prime}(x)(x + 1)^{2}  \\
\mu^{\prime}(x)  & = \sqrt[]{ x + 1 } \\
\mu(x) & = \frac{2}{3}(x + 1)^{3/2} 
\end{align}
$$

则$y^{*} = \frac{2}{3}(x + 1)^{7/2}$

通解为
$$
y + y^{*} = C(x + 1)^{2} +\frac{2}{3}(x + 1)^{7/2} 
$$

> [!Question] 例题
> 求通解$y^{\prime} + y\tan x = \sec x$

先求齐次方程通解
$$
\begin{align}
y^{\prime} + y\tan x  & = 0  \\
y^{\prime}  & = -y\tan x \\
\frac{1}{y} dy & =  -\tan x dx \\
\ln y  & = \ln |\cos x|  +C_{1} \\
y  &  = C_{1}\cos x 
\end{align}
$$
令$y^{*}(x) = C_{1}(x)\cos x$
则$y^{\prime *}(x)= C_{1}^{\prime}(x)\cos x -C_{1}(x)\sin x$
代入方程
$$
\begin{align}
C_{1}^{\prime}(x)\cos x = \sec x \\
C_{1}^{\prime}(x) = \sec ^{2}x  \\
C_{1}(x) = \tan x + C
\end{align}
$$
则$y^{*}(x)=(\tan x +C)\cos x$
通解为
$$
\begin{align}
y  & = (\tan x + C_{1}) \cos x \\
 & = \sin x + C_{1} \cos x
\end{align}
$$

#### 代公式

> [!Question] 例题
> 求通解$xy^{\prime}\ln x + y = ax(1 + \ln x)$

$$
\begin{align}
y^{\prime} +\frac{1}{x\ln x}y = \frac{a(1  + \ln x)}{\ln x}  \\
y^{\prime} +\frac{1}{x\ln x}y =a + \frac{a}{\ln x}
\end{align}
$$
$$
\begin{cases}
P(x) = \frac{1}{x\ln x} \\
Q(x) = a + \frac{a}{\ln x}
\end{cases}
$$
通解公式：
$$
\begin{align}
Ce^{-\int P(x)dx} + \int Q(x)e^{\int P(x)dx} dx \\
\end{align}
$$
$$
\begin{align}
\int P(x) dx  &  = \int \frac{1}{x \ln x}dx \\
 & = \int_{1}  \frac{1}{\ln x}d(\ln x) \\
 & = \ln \ln x
\end{align}
$$
则
$$
\begin{align}
 & Ce^{-\int P(x)dx} + e^{-\int P(x)dx}\int Q(x)e^{\int P(x)dx} dx  \\
 & =  Ce^{-\ln \ln x} + e^{-\ln \ln x}\int \left( a + \frac{a}{\ln x} \right)e^{\ln \ln x} \\
 & = \frac{C}{\ln x} + \frac{1}{\ln x}\int (a\ln x + a )dx \\
 & = \frac{1}{\ln x}\left( C + ax + ax\ln x - \int x d(a\ln x) \right) \\
 & =\frac{1}{\ln x} \left( C + ax + ax\ln x -a \int dx \right) \\
 & =\frac{1}{ \ln x}(C+ ax + ax\ln x -ax) \\
 & = \frac{1}{ \ln x}(C+ ax\ln x)
\end{align}
$$

#### 自变量与因变量交换
求通解$(x - 2xy - y^{2})\frac{dy}{dx} + y^{2} = 0$

$$
\begin{align}
y^{2} = (y^{2} + 2xy - x) \frac{dy}{dx} \\
\frac{dx}{dy}y^{2} = y^{2} + 2xy - x \\
\frac{dx}{dy} =1 + \frac{2x}{y} - \frac{x}{y^{2}} \\
\frac{dx}{dy} +\left( \frac{1}{y^{2}}  - \frac{2}{y}\right)x = 1
\end{align}
$$
有
$$
\begin{align}
P(y) =\frac{1}{y^{2}} - \frac{2}{y} \\
Q(y) = 1
\end{align}
$$


$$
x = e^{-\int P(y) dy}\left( \int Q(y)e^{\int P(y)dy} dy + C \right)
$$

$$
\begin{align}
\int P(y)dy  & =\int \left( \frac{1}{y^{2}} -\frac{2}{y} \right)dy \\
 & =-\frac{1}{y}-2\ln y
\end{align}
$$
$$
\begin{align}
x   & = e^{\frac{1}{y}+ 2\ln y} \left( \int Q(y)e^{-\frac{1}{y}-2\ln y}dy  +C \right)  \\
 & =y^{2}e^{\frac{1}{y} } \left( \int y^{-2}e^{-\frac{1}{y}} dy + C \right) \\
 & = Cy^{2}e^{\frac{1}{y} } + y^{2}e^{\frac{1}{y} }\int  d(e^{-\frac{1}{y}}) \\
 & = Cy^{2}e^{\frac{1}{y} } + y^{2}
\end{align}
$$

连续函数$f(x)$满足$f(x) = \int_{0}^{3x} f\left( \frac{t}{3} \right) \, dt + e^{2x}$，求$f(x)$

对上式求导
$$
\begin{align}
y^{\prime} =3f(x) + 2e^{2x} \\
\frac{dy}{dx} - 3y = 2e^{2x}
\end{align}
$$
$$
\begin{cases}
P(x) = -3 \\
Q(x) = 2e^{2x}
\end{cases}
$$
通解为
$$
y  = e^{- \int P(x)dx}\left( \int Q(x)e^{\int P(x)dx}dx + C \right)
$$

$$
\int P(x)dx = -3x
$$
$$
\begin{align}
y  & = e^{3x }\left( \int 2e^{2x}(e^{-3x})dx + C \right) \\
 & =e^{3x }\left( \int 2e^{-x}dx + C  \right)\\
 & =-2e^{3x}(e^{-x}) + Ce^{3x} \\
 & = -2e^{2x} + Ce^{3x}
\end{align}
$$

当$x=0$，有$y = 1$
则
$$
\begin{align}
1 = -2 + C \\
C = 3
\end{align}
$$
则
$$
f(x) = -2e^{2x} + 3e^{3x}
$$

#### 伯努利方程

形式：$\frac{dy}{dx} + P(x)y = Q(x)y^{n}$


> [!Question] 例题
> 求通解$\frac{dy}{dx} + \frac{y}{x} = a \ln x y^{2}$

$$
\begin{align}
\frac{1}{y^{2}} \frac{dy}{dx} + \frac{1}{xy} + a\ln x
\end{align}
$$
令$z = \frac{1}{y} , dz = -\frac{1}{y^{2}} dy$ 
$$
\begin{align}
-\frac{dz}{dx} +  \frac{z}{x} =  a\ln x \\
\frac{dz}{dx}  - \frac{z}{x} = -a \ln x \\
\end{align}
$$

令
$$
\begin{align}
\frac{dz}{dx} & = \frac{z}{x} \\
\frac{1}{z}dz &  = \frac{1}{x}dx \\
\ln x & = \ln x  + \ln C \\
z &  = Cx \\
\end{align}
$$
令$z = \mu(x)x$
$z^{\prime} = \mu^{\prime}(x)x + \mu(x)$
代入$\frac{dz}{dx}  - \frac{z}{x} = -a \ln x$

$$
\begin{align}
\mu^{\prime}(x)x = -a\ln x \\
\mu^{\prime} (x) = -\frac{a\ln x}{x}  \\
\mu(x)= -\frac{a(\ln x)^{2}}{2} + C
\end{align}
$$

$$
\begin{align}
z  & = ( C - a(\ln x)^{2} )x \\
\frac{1}{y} & = (C-a(\ln x)^{2})x \\
xy(C-a(\ln x)^{2}) &  = 1
\end{align}
$$


> [!Question] 例题
> 求通解$2xy^{3}y^{\prime} + x^{4} - y^{4} = 0$

$$
\begin{align}
y^{\prime} + \frac{x^{3}}{2y^{3}} - \frac{y}{2x}& = 0  \\
\frac{dy}{dx} - \frac{1}{2x}y  & = \frac{x^{3}}{2}y^{-3} \\
y^{3} \frac{dy}{dx} - \frac{1}{2x}y^{4} & =\frac{x^{3}}{2}
\end{align}
$$

令$z = y^{4} , dz = 4y^{3}dy$
$$
\begin{align}
\frac{1}{4} \frac{dz}{dx} - \frac{z}{2x} = \frac{x^{3}}{2} \\
\frac{dz}{dx} - \frac{2z}{x} =  2x^{3}
\end{align}
$$
令
$$
\begin{align}
\frac{dz}{dx} & = \frac{2z}{x} \\
\frac{1}{z}dz & = \frac{2}{x}dx \\
\ln |z| & = 2\ln |x| + \ln C \\
z  & = Cx^{2}
\end{align}
$$
令$z = \mu(x)x^{2}$
则$z^{\prime} =\mu^{\prime}(x)x^{2} + 2x\mu(x)$

$$
\begin{align}
\mu^{\prime}(x)x^{2} = 2x^{3} \\
\mu^{\prime}(x) = 2x \\
\mu(x) = x^{2} + C
\end{align}
$$
则
$$
\begin{align}
z =(x^{2} + C)x^{2} \\
y^{4} - x^{4} -Cx^{2} =0
\end{align}
$$

