---
{"dg-publish":true,"permalink":"/Advanced Math 高等数学/4_微分中值定理/例题：泰勒展开/","tags":["例题","微积分","高数"]}
---


> [!Question] 问题
> 求麦克劳林公式，并求$y^{(n)}0$
> $$
> y = \frac{1 - 2x + 5x^{2}}{(1-2x)(1 + x^{2})}
> $$


已知
$$
\begin{align}
\frac{1}{1+x}  & = 1 - x + x^{2} - x^{3} + \dots +(-1)^{n}x^{n} +o(x^{n})\\
\frac{1}{1-x}  & = 1 + x + x^{2} + x^{3} + \dots +x^{n} +o(x^{n})
\end{align}
$$
则
$$
\frac{1}{1-2x} = 1 + 2x + 4x^{2} + 8x^{3} + \dots + (2x)^{n} +o(x^{n})
$$

$$
\frac{1}{1+ x^{2}} = 1 -x^{2} + x^{4}+ \dots  +(-1)^{n}x^{2n}+o(x^{2n})
$$
  对原式做分解
  $$
  \begin{align}
y  & = \frac{1 - 2x + 5x^{2}}{(1-2x)(1 + x^{2})} \\
 & =\frac{(1+ x^{2})-2x(1-2x)}{(1- 2x)(1 + x^{2})} \\
 & = \frac{1}{1-2x}-\frac{2x}{1 + x^{2}}
\end{align}
$$

则经过泰勒展开变为
$$
\begin{align}
y  & = 1 + 2x + 4x^{2} + 8x^{3} + \dots + (2x)^{2n} +o(x^{2n}) + 2x(1 -x^{2} + x^{4}+ \dots  +(-1)^{n}x^{2n}+o(x^{n})) \\
y  & = 1 + 2x + 4x^{2} + 8x^{3} + \dots + (2x)^{2n} +o(x^{n}) + 2x - 2x^{3} + 2x^{5}+ \dots + (-1)^{n}2x^{2n+1}
\end{align}
$$
$$
\frac{y^{n}(0)}{n!} = \begin{cases}
2^{n} ,n = 2k \\
2^{n} + 2, n = 4k + 1 \\
2^{n} - 2, n = 4k + 3
\end{cases}
$$
因此
$$
y^{(n)}(0) = \begin{cases}
2^{n}n! ,n = 2k \\
(2^{n} + 2)n!, n = 4k + 1 \\
(2^{n} - 2)n!, n = 4k + 3
\end{cases}
$$

> [!Question] 问题
> 求麦克劳林公式，并求$y^{(n)}0$
> $$
> y = \ln(x + \sqrt[]{ 1 + x^{2} })
> $$

注意到
$$
y^{\prime} = \frac{1}{x + \sqrt[]{ 1 + x^{2} }}\left( 1 + \frac{1}{2\sqrt[]{ 1 +x^{2} }}2x \right) = \frac{1}{\sqrt[]{ 1 + x^{2} }}

$$

而$\frac{1}{\sqrt[]{ 1 + x^{2} }}$的麦克劳林公式为
$$
\begin{align}
(1 + x^{2})^{-1/2}  & = 1 -\left( \frac{1}{2} \right)x^{2} + \frac{\left( -\frac{1}{2} \right)\left( -\frac{3}{2} \right)}{2}x^{4} + \dots + \frac{\left( -\frac{1}{2} \right)\left( -\frac{3}{2} \right)\dots\left( -\frac{2n-1}{2} \right)}{n!}x^{2n} + o(x^{2n-1}) \\
(1 + x^{2})^{-1/2}  & = 1 - \frac{x^{2}}{2} + \frac{3}{8}x^{4}+ \dots + \frac{(-1)^{n}(2n-1)!!}{2^{n}(n!)}x^{2n}  +o(x^{2n+1})
\end{align}
$$
则有
$$
\begin{align}
\frac{y^{\prime(n)}(0)}{n!} = \begin{cases}
0 , n  = 2k+1 \\
\frac{(-1)^{n/2}(n-1)!!}{2^{n/2}\left( \frac{n}{2} \right)!} , n = 2k
\end{cases}  \\
y^{(n + 1)}(0) = \begin{cases}
0 , n  = 2k+1 \\
\frac{(-1)^{n/2}(n-1)!!n!}{2^{n/2}\left( \frac{n}{2} \right)!} , n = 2k
\end{cases}  \\
y^{n}(0) = \begin{cases}
0 , n  = 2k \\
\frac{(-1)^{(n-1)/2}(n-2)!!n-1!}{2^{(n-1)/2}\left( \frac{n-1}{2} \right)!} , n = 2k + 1
\end{cases} 
\end{align}
$$
则$y = \ln(x + \sqrt[]{ 1 + x^{2} })$的多项式系数为
$$
\frac{y^{(n)}(0)}{n!} = \begin{cases}
0 , n  = 2k \\
\frac{(-1)^{(n-1)/2}(n-2)!!}{2^{(n-1)/2}\left( \frac{n-1}{2} \right)!n} , n = 2k + 1
\end{cases} 
$$
则有
$$
\ln(x + \sqrt[]{ 1 + x^{2} }) =  x - \frac{x^{3}}{3} + \frac{3x^{5}}{40} + \dots + \frac{(-1)^{n}(2n -1)!!}{2^{n}(n!)(2n+1)}x^{2n + 1}
$$

